Add wfv to calls_correct and prove cheat in App case
The theorem statement is now annoyingly intricate, since certain
assumptions are required for parts of the conclusion, but are too strong
for the inductive hypothesis in general. The alternative would be to
prove two theorems, but they would have duplicated a lot of proof.

The ev_app cases have not been updated (broken and commented out).

compiler/backend/proofs/clos_callProofScript.sml
@@ -188,6 +188,12 @@ val wfv_def = tDefine"wfv"`
    rpt strip_tac >> imp_res_tac v_size_lemma >> simp[]);
 val _ = export_rewrites["wfv_def"];
 
+val wfv_state_def = Define`
+  wfv_state g l s ⇔
+    EVERY (OPTION_EVERY (wfv g l)) s.globals ∧
+    FEVERY (every_refv (wfv g l) o SND) s.refs ∧
+    s.code = FEMPTY`;
+
 val state_rel_def = Define`
   state_rel g l (s:'ffi closSem$state) (t:'ffi closSem$state) ⇔
     (s.ffi = t.ffi) ∧
@@ -1149,6 +1155,20 @@ val dest_closure_v_rel = Q.store_thm("dest_closure_v_rel",
   \\ first_x_assum(qspecl_then[`x`,`n`]mp_tac)
   \\ simp[]);
 
+val dest_closure_wfv = Q.store_thm("dest_closure_wfv",
+  `dest_closure loco v env = SOME (Partial_app x) ∧
+   EVERY (wfv g l) env ∧ wfv g l v ⇒ wfv g l x`,
+  rw[dest_closure_def]
+  \\ every_case_tac \\ fs[]
+  \\ rw[]
+  \\ rpt(pairarg_tac \\ fs[])
+  \\ every_case_tac \\ fs[]
+  \\ (qmatch_asmsub_rename_tac`Closure lopt` ORELSE
+      qmatch_asmsub_rename_tac`Recclosure lopt`)
+  \\ Cases_on`lopt` \\ fs[] \\ rveq
+  \\ fsrw_tac[ETA_ss][]
+  \\ metis_tac[]);
+
 val env_rel_DROP = Q.store_thm("env_rel_DROP",
   `env_rel R (DROP x l1) (DROP x l2) x es ∧
    LIST_REL R (TAKE x l1) (TAKE x l2) ∧
@@ -1401,51 +1421,44 @@ val v_rel_Boolv = store_thm("v_rel_Boolv[simp]",
   ``v_rel g1 l1 (Boolv b) v <=> (v = Boolv b)``,
   Cases_on `b` \\ Cases_on `v` \\ fs [v_rel_def,Boolv_def]);
 
+val s0 = ``s0:'ffi closSem$state``;
+
 (* compiler correctness *)
 
 val calls_correct = Q.store_thm("calls_correct",
-  `(∀tmp xs env1 (s0:'ffi closSem$state) g0 g env2 t0 ys res s l l1 g1.
+  `(∀tmp xs env1 ^s0 g0 g env2 t0 ys res s l l1 g1.
     tmp = (xs,env1,s0) ∧
     evaluate (xs,env1,s0) = (res,s) ∧
     res ≠ Rerr (Rabort Rtype_error) ∧
     calls xs g0 = (ys,g) ∧
-    every_Fn_SOME xs ∧ every_Fn_vs_NONE xs ∧
-    set (code_locs xs) ⊆ EVEN ∧
-    (*
-    EVERY (wfv g1 l1) env1 ∧
-    EVERY (OPTION_EVERY (wfv g1 l1)) s0.globals ∧
-    FEVERY (every_refv (wfv g1 l1) o SND) s0.refs ∧
-    *)
+    every_Fn_SOME xs ∧ every_Fn_vs_NONE xs ∧ set (code_locs xs) ⊆ EVEN ∧
+    EVERY (wfv g1 l1) env1 ∧ wfv_state g1 l1 s0 ∧
     wfg g0 ∧
     ALL_DISTINCT (code_locs xs) ∧
     DISJOINT (IMAGE SUC (set (code_locs xs))) (set (MAP FST (SND g0))) ∧
     l = set (code_locs xs) DIFF domain (FST g) ∧
-    env_rel (v_rel g1 l1) env1 env2 0 (MAP (λx. (0,x)) ys) ∧
-    state_rel g1 l1 s0 t0 ∧
-    subg g g1 ∧ l ⊆ l1 ∧ DISJOINT l1 (domain (FST g1)) ∧ wfg g1 ∧
-    code_includes (SND g) t0.code
+    subg g g1 ∧ l ⊆ l1 ∧ DISJOINT l1 (domain (FST g1)) ∧ wfg g1
     ⇒
     ∃ck res' t.
-    evaluate (ys,env2,t0 with clock := t0.clock + ck) = (res',t) ∧
-    state_rel g1 l1 s t ∧
-    result_rel (LIST_REL (v_rel g1 l1)) (v_rel g1 l1) res res' (* ∧
-    every_result (EVERY (wfv g1 l1)) (wfv g1 l1) res ∧
-    EVERY (OPTION_EVERY (wfv g1 l1)) s.globals ∧
-    FEVERY (every_refv (wfv g1 l1) o SND) s.refs *)
-    ) ∧
-  (∀loco f args (s0:'ffi closSem$state) loc g l t0 res s f' args'.
+    every_result (EVERY (wfv g1 l1)) (wfv g1 l1) res ∧ wfv_state g1 l1 s ∧
+    (env_rel (v_rel g1 l1) env1 env2 0 (MAP (λx. (0,x)) ys) ∧
+     state_rel g1 l1 s0 t0 ∧ code_includes (SND g) t0.code ⇒
+     evaluate (ys,env2,t0 with clock := t0.clock + ck) = (res',t) ∧
+     state_rel g1 l1 s t ∧
+     result_rel (LIST_REL (v_rel g1 l1)) (v_rel g1 l1) res res')) ∧
+  (∀loco f args ^s0 loc g l t0 res s f' args'.
     evaluate_app loco f args s0 = (res,s) ∧
     res ≠ Rerr (Rabort Rtype_error) ∧
-    v_rel g l f f' ∧
-    (* check_args_if_call (domain (FST g)) f (LENGTH args) ∧ *)
-    LIST_REL (v_rel g l) args args' ∧
-    state_rel g l s0 t0 ∧
+    wfv g l f ∧ EVERY (wfv g l) args ∧ wfv_state g l s0 ∧
     wfg g ∧ DISJOINT l (domain (FST g))
     ⇒
     ∃ck res' t.
-    evaluate_app loco f' args' (t0 with clock := t0.clock + ck) = (res',t) ∧
-    state_rel g l s t ∧
-    result_rel (LIST_REL (v_rel g l)) (v_rel g l) res res')`,
+    every_result (EVERY (wfv g l)) (wfv g l) res ∧ wfv_state g l s ∧
+    (v_rel g l f f' ∧ LIST_REL (v_rel g l) args args' ∧
+     state_rel g l s0 t0 ⇒
+     evaluate_app loco f' args' (t0 with clock := t0.clock + ck) = (res',t) ∧
+     state_rel g l s t ∧
+     result_rel (LIST_REL (v_rel g l)) (v_rel g l) res res'))`,
   ho_match_mp_tac evaluate_ind
   \\ conj_tac
   >- (
@@ -1454,6 +1467,7 @@ val calls_correct = Q.store_thm("calls_correct",
     \\ fs[calls_def,evaluate_def]
     \\ rveq \\ fs[evaluate_def]
     \\ fs[code_locs_def]
+    \\ simp[RIGHT_EXISTS_IMP_THM]
     \\ metis_tac[state_rel_subg,SUBSET_REFL])
   \\ conj_tac >- cheat
    (*
@@ -1535,7 +1549,7 @@ val calls_correct = Q.store_thm("calls_correct",
     \\ every_case_tac
     \\ imp_res_tac LIST_REL_LENGTH \\ fs []
     \\ qexists_tac `0` \\ fs []
-    \\ fs [LIST_REL_EL_EQN])
+    \\ fs [LIST_REL_EL_EQN,EVERY_MEM,MEM_EL,PULL_EXISTS,RIGHT_EXISTS_IMP_THM])
   (* If *)
   \\ conj_tac >- cheat
    (*
@@ -1863,20 +1877,21 @@ val calls_correct = Q.store_thm("calls_correct",
     \\ strip_tac \\ rveq
     \\ fs[PULL_EXISTS]
     \\ qexists_tac`0`
-    \\ simp[v_rel_def,recclosure_rel_def]
-    \\ fs[code_locs_def,IN_EVEN]
-    \\ imp_res_tac calls_length
-    \\ fs[quantHeuristicsTheory.LIST_LENGTH_2] \\ rveq
-    \\ fsrw_tac[ETA_ss][PULL_EXISTS,calls_list_def]
-    \\ fs[closed_Fn]
-    \\ `subg g0 (insert_each x 1 g0)`
-    by ( simp[subg_def,insert_each_subspt] \\ fs[wfg_def])
+    \\ fsrw_tac[ETA_ss][]
     \\ CONV_TAC(RESORT_EXISTS_CONV(sort_vars["g0'"]))
     \\ qexists_tac`g0` \\ fs[]
-    \\ fs[ALL_DISTINCT_APPEND]
+    \\ qmatch_asmsub_abbrev_tac`COND b`
+    \\ CONV_TAC(RESORT_EXISTS_CONV(sort_vars["fns2"]))
+    \\ qexists_tac`if b then calls_list x [(num_args,exp)] else [(num_args,HD e1')]` \\ fs[]
+    \\ simp[PULL_EXISTS,GSYM RIGHT_EXISTS_IMP_THM]
+    \\ simp[RIGHT_EXISTS_AND_THM]
+    \\ imp_res_tac calls_length \\ fs[quantHeuristicsTheory.LIST_LENGTH_2]
+    \\ fs[closed_Fn,code_locs_def,IN_EVEN,GSYM ADD1,ALL_DISTINCT_APPEND]
+    \\ `subg g0 (insert_each x 1 g0)`
+    by ( simp[subg_def,insert_each_subspt] \\ fs[wfg_def])
     \\ `wfg g`
     by (
-      reverse every_case_tac \\ fs[] \\ rw[]
+      qunabbrev_tac`b` \\ reverse every_case_tac \\ fs[] \\ rw[]
       >- ( match_mp_tac calls_wfg \\ asm_exists_tac \\ fs[] )
       \\ qpat_assum`calls _ (insert_each _ _ _) = _`assume_tac
       \\ drule calls_wfg'
@@ -1907,19 +1922,25 @@ val calls_correct = Q.store_thm("calls_correct",
       \\ imp_res_tac calls_subspt
       \\ imp_res_tac subspt_domain_SUBSET
       \\ fs[domain_FST_insert_each] )
-    \\ CASE_TAC \\ fs[] \\ rveq
-    \\ simp[evaluate_def]
-    \\ fs[DISJOINT_SYM]
-    \\ imp_res_tac calls_add_SUC_code_locs
-    \\ fs[SUBSET_DEF,GSYM ADD1,recclosure_wf_def]
-    \\ rpt conj_tac
-    \\ TRY (Cases_on`new_g'` \\ fs[code_list_def,GSYM ADD1] \\ NO_TAC)
-    \\ TRY (
-      first_x_assum match_mp_tac
+    \\ conj_asm1_tac
+    >- (
+      fs[recclosure_rel_def,recclosure_wf_def,GSYM ADD1]
+      \\ CASE_TAC \\ fs[calls_list_MAPi] \\ rveq
+      \\ imp_res_tac calls_add_SUC_code_locs
+      \\ fs[SUBSET_DEF]
+      \\ fs[RIGHT_EXISTS_IMP_THM,GSYM AND_IMP_INTRO]
+      \\ rpt conj_tac
+      \\ TRY (Cases_on`new_g'` \\ fs[code_list_def,GSYM ADD1] \\ NO_TAC)
+      \\ first_x_assum (match_mp_tac o MP_CANON)
       \\ rfs[wfg_def,PULL_EXISTS]
       \\ metis_tac[] )
-    \\ fs[env_rel_def,fv1_thm,fv_GENLIST_Var]
-    \\ rw[] \\ imp_res_tac calls_fv_imp \\ fs[])
+    \\ simp[v_rel_def,PULL_EXISTS,GSYM RIGHT_EXISTS_IMP_THM]
+    \\ fsrw_tac[ETA_ss][]
+    \\ simp[RIGHT_EXISTS_IMP_THM]
+    \\ Cases_on`b` \\ fs[] \\ rveq \\ simp[evaluate_def]
+    \\ fs[calls_list_def,GSYM ADD1] \\ strip_tac
+    \\ asm_exists_tac \\ fs[]
+    \\ fs[env_rel_def,fv1_thm,fv_GENLIST_Var])
   (* Letrec *)
   \\ conj_tac >- cheat
   (* App *)
@@ -1950,10 +1971,10 @@ val calls_correct = Q.store_thm("calls_correct",
     by (
       match_mp_tac calls_wfg
       \\ asm_exists_tac \\ fs[] )
-    \\ `env_rel (v_rel g1 l1) env env2 0 (MAP (λx. (0,x)) es)`
+    \\ `env_rel (v_rel g1 l1) env env2 0 (MAP (λx. (0,x)) ys) ⇒
+        env_rel (v_rel g1 l1) env env2 0 (MAP (λx. (0,x)) es)`
     by (
-      qhdtm_x_assum`env_rel`mp_tac
-      \\ qpat_assum`_ = (ys,_)`mp_tac
+      qpat_assum`_ = (ys,_)`mp_tac
       \\ qmatch_goalsub_abbrev_tac`COND b1`
       \\ reverse(Cases_on`b1`) \\ fs[]
       >- (
@@ -1972,11 +1993,11 @@ val calls_correct = Q.store_thm("calls_correct",
       strip_tac \\ rveq \\ rfs[]
       \\ first_x_assum drule \\ fs[DISJOINT_SYM,ALL_DISTINCT_APPEND]
       \\ rpt(disch_then drule)
+      \\ disch_then(qspecl_then[`env2`,`t0`]mp_tac)
       \\ impl_tac
       >- (
         conj_tac >- metis_tac[subg_trans]
         \\ simp[]
-        \\ reverse conj_tac >- metis_tac[code_includes_subg]
         \\ fs[SUBSET_DEF]
         \\ fs[subg_def]
         \\ imp_res_tac subspt_domain_SUBSET
@@ -1989,10 +2010,13 @@ val calls_correct = Q.store_thm("calls_correct",
       \\ strip_tac
       \\ qexists_tac`ck`
       \\ imp_res_tac calls_length
-      \\ `state_rel g1 l1 r t`
+      \\ simp[RIGHT_EXISTS_AND_THM,RIGHT_EXISTS_IMP_THM]
+      \\ strip_tac
+      \\ `state_rel g1 l1 r t ∧ code_includes (SND g') t0.code`
       by (
         imp_res_tac evaluate_const \\ fs[]
-        \\ metis_tac[state_rel_subg] )
+        \\ metis_tac[state_rel_subg,code_includes_subg] )
+      \\ fs[] \\ rfs[] \\ rveq
       \\ `exc_rel (v_rel g1 l1) e e'`
       by ( Cases_on`e`\\fs[] \\ metis_tac[v_rel_subg])
       \\ every_case_tac \\ fs[] \\ rw[evaluate_def]
@@ -2004,11 +2028,11 @@ val calls_correct = Q.store_thm("calls_correct",
     \\ first_x_assum drule \\ fs[DISJOINT_SYM]
     \\ fs[ALL_DISTINCT_APPEND]
     \\ rpt(disch_then drule)
+    \\ disch_then(qspecl_then[`env2`,`t0`]mp_tac)
     \\ impl_tac
     >- (
       conj_tac >- metis_tac[subg_trans]
       \\ simp[]
-      \\ reverse conj_tac >- metis_tac[code_includes_subg]
       \\ fs[SUBSET_DEF]
       \\ fs[subg_def]
       \\ imp_res_tac subspt_domain_SUBSET
@@ -2037,31 +2061,44 @@ val calls_correct = Q.store_thm("calls_correct",
       \\ impl_tac
       >- (
         imp_res_tac evaluate_const \\ fs[]
-        \\ fs[SUBSET_DEF]
-        \\ fs[env_rel_def,fv1_thm]
-        \\ metis_tac[] )
+        \\ fs[SUBSET_DEF])
       \\ strip_tac
       \\ reverse BasicProvers.TOP_CASE_TAC \\ fs[]
       >- (
         strip_tac \\ rveq \\ fs[]
+        \\ simp[RIGHT_EXISTS_IMP_THM,RIGHT_EXISTS_AND_THM]
+        \\ strip_tac \\ fs[] \\ rfs[]
+        \\ `code_includes (SND g') t0.code` by metis_tac[code_includes_subg] \\ fs[]
         \\ qpat_assum`evaluate(es,env2,_) = _`(mp_tac o MATCH_MP evaluate_add_clock)
         \\ disch_then(qspec_then`ck'`mp_tac) \\ simp[] \\ strip_tac
         \\ qexists_tac`ck+ck'` \\ fs[]
-        (*
-        \\ imp_res_tac evaluate_const \\ fs[]
-        \\ conj_tac >- metis_tac[state_rel_subg]
-        \\ Cases_on`e` \\ fs[]
-        \\ metis_tac[v_rel_subg]*))
+        \\ qpat_assum`_ ⇒ _`mp_tac
+        \\ impl_tac
+        >- (
+          imp_res_tac evaluate_const \\ fs[]
+          \\ fs[env_rel_def,fv1_thm]
+          \\ metis_tac[] )
+        \\ strip_tac \\ fs[])
       \\ strip_tac \\ fs[] \\ rfs[]
       \\ imp_res_tac evaluate_length_imp
       \\ fs[quantHeuristicsTheory.LIST_LENGTH_2]
       \\ rveq \\ fs[]
       \\ first_x_assum drule
+      \\ rpt(disch_then drule)
+      \\ simp[RIGHT_EXISTS_IMP_THM,RIGHT_EXISTS_AND_THM,FORALL_AND_THM]
+      \\ strip_tac \\ fs[] \\ strip_tac \\ fs[] \\ rfs[]
+      \\ `code_includes (SND g') t0.code` by metis_tac[code_includes_subg] \\ fs[]
+      \\ qpat_assum`_ ⇒ _`mp_tac
+      \\ impl_tac
+      >- (
+        imp_res_tac evaluate_const \\ fs[]
+        \\ fs[env_rel_def,fv1_thm]
+        \\ metis_tac[] )
+      \\ strip_tac \\ fs[] \\ rveq
+      \\ first_x_assum drule
+      \\ rpt(disch_then drule)
+      \\ strip_tac
       \\ qmatch_assum_rename_tac`LIST_REL (v_rel _ _) ev1 ev2`
-      \\ disch_then drule
-      \\ disch_then drule
-      \\ impl_tac >- rw[]
-      \\ strip_tac \\ simp[]
       \\ qpat_assum`evaluate(es,env2,_) = _`(mp_tac o MATCH_MP evaluate_add_clock)
       \\ disch_then(qspec_then`ck'+ck''`mp_tac) \\ simp[] \\ strip_tac
       \\ qpat_assum`evaluate([_],env2,_) = _`(mp_tac o MATCH_MP evaluate_add_clock)
@@ -2087,6 +2124,18 @@ val calls_correct = Q.store_thm("calls_correct",
       \\ ntac 2 strip_tac \\ rveq
       \\ fs[quantHeuristicsTheory.LIST_LENGTH_2] \\ rveq
       \\ rfs[] \\ rveq
+      \\ qpat_assum`_ ⇒ _`mp_tac
+      \\ impl_tac >- fs[SUBSET_DEF]
+      \\ strip_tac \\ fs[]
+      \\ first_x_assum drule
+      \\ simp[RIGHT_EXISTS_IMP_THM,RIGHT_EXISTS_AND_THM,FORALL_AND_THM]
+      \\ strip_tac \\ fs[]
+      \\ strip_tac \\ fs[]
+      \\ qpat_assum`_ ⇒ _`kall_tac
+      \\ qpat_assum`_ ⇒ _`mp_tac
+      \\ impl_keep_tac
+      >- ( fs[] \\ metis_tac[code_includes_subg] )
+      \\ strip_tac \\ fs[]
       \\ qmatch_assum_rename_tac`LIST_REL (v_rel g1 l1) ev1 ev2`
       \\ Cases_on`ev1 = []`
       \\ imp_res_tac evaluate_length_imp \\ rfs[]
@@ -2096,7 +2145,8 @@ val calls_correct = Q.store_thm("calls_correct",
       \\ strip_tac
       \\ drule (GEN_ALL dest_closure_v_rel_lookup)
       \\ qmatch_assum_rename_tac`dest_closure _ f1 ev1 = _`
-      \\ `∃f2. v_rel g1 l1 f1 f2` by cheat
+      \\ `∃f2. v_rel g1 l1 f1 f2`
+      by ( match_mp_tac v_rel_exists \\ fs[] )
       \\ disch_then drule
       \\ disch_then drule
       \\ impl_tac >- rw[]
@@ -2115,6 +2165,7 @@ val calls_correct = Q.store_thm("calls_correct",
         \\ rpt(first_x_assum drule)
         \\ simp[] )
       \\ rfs[]
+      \\ qpat_assum`code_includes (SND g) _`assume_tac
       \\ drule (GEN_ALL code_includes_ALOOKUP)
       \\ disch_then drule \\ strip_tac
       \\ `t.code = t0.code` by (imp_res_tac evaluate_const \\ fs[])
@@ -2122,12 +2173,11 @@ val calls_correct = Q.store_thm("calls_correct",
       \\ disch_then drule
       \\ qpat_assum`state_rel g1 l1 r t`assume_tac
       \\ disch_then drule
-      \\ impl_tac >- rw[]
       \\ strip_tac
       \\ imp_res_tac LIST_REL_LENGTH \\ fs[]
       \\ Cases_on`ev2 = []` \\ fs[]
       \\ fs[evaluate_app_rw]
-      \\ qpat_assum`_ = (res',_)`mp_tac
+      \\ qpat_assum`_ = (_,_)`mp_tac
       \\ imp_res_tac state_rel_clock \\ fs[]
       \\ IF_CASES_TAC \\ fs[]
       >- (
@@ -2138,16 +2188,13 @@ val calls_correct = Q.store_thm("calls_correct",
       \\ simp[evaluate_def,evaluate_GENLIST_Var]
       \\ simp[find_code_def]
       \\ simp[Once dec_clock_def]
-      (*
-      \\ `t'.code = t.code` by (imp_res_tac evaluate_const \\ fs[])
-      *)
       \\ fs[]
       \\ simp[Once dec_clock_def]
       \\ imp_res_tac evaluate_length_imp \\ fs[NOT_LESS]
       \\ IF_CASES_TAC
       >- (
         fs[] \\ strip_tac \\ rveq \\ fs[]
-        \\ `t.clock = LENGTH ev2 - ck'` by decide_tac
+        \\ `t.clock = LENGTH ev2 - ck''` by decide_tac
         \\ fs[]
         \\ qexists_tac`ck` \\ simp[]
         \\ fs[dec_clock_def])
@@ -2155,33 +2202,18 @@ val calls_correct = Q.store_thm("calls_correct",
       \\ strip_tac
       \\ fs[dec_clock_def,TAKE_APPEND1]
       \\ qpat_assum`evaluate(es,env2,_) = _`(mp_tac o MATCH_MP evaluate_add_clock)
-      \\ disch_then(qspec_then`ck'`mp_tac) \\ simp[] \\ strip_tac
-      \\ qexists_tac`ck+ck'` \\ simp[]
-      \\ qpat_assum`_ = (res',_)`mp_tac
+      \\ disch_then(qspec_then`ck''`mp_tac) \\ simp[] \\ strip_tac
+      \\ qexists_tac`ck+ck''` \\ simp[]
+      \\ qpat_assum`_ _  _ = (_,_)`mp_tac
       \\ BasicProvers.TOP_CASE_TAC \\ fs[]
       \\ BasicProvers.TOP_CASE_TAC \\ fs[]
       \\ TRY BasicProvers.TOP_CASE_TAC \\ fs[]
-      \\ strip_tac \\ rveq \\ fs[]
-      \\ TRY (Cases_on`res`\\fs[])
-      \\ rveq \\ fs[]
-      \\ TRY (
-        pop_assum mp_tac \\ CASE_TAC \\ fs[]
-        \\ strip_tac \\ rveq \\ fs[] \\ rveq \\ fs[])
-      \\ imp_res_tac evaluate_const \\ fs[]
-      \\ rpt conj_tac
-      \\ TRY(match_mp_tac (GEN_ALL state_rel_subg))
-      \\ TRY(match_mp_tac (GEN_ALL (MP_CANON LIST_REL_mono)))
-      \\ TRY (Cases_on`e''` \\ fs[])
-      \\ metis_tac[v_rel_subg])
+      \\ TRY BasicProvers.TOP_CASE_TAC \\ fs[])
     \\ qpat_assum`_ ⇒ _`mp_tac
     \\ impl_tac
     >- (
       imp_res_tac evaluate_const \\ fs[]
-      \\ fs[SUBSET_DEF]
-      \\ fsrw_tac[ETA_ss][env_rel_def,fv1_thm,EXISTS_MAP,fv_exists]
-      \\ imp_res_tac calls_length \\ fs[quantHeuristicsTheory.LIST_LENGTH_2]
-      \\ rveq \\ fs[]
-      \\ metis_tac[] )
+      \\ fs[SUBSET_DEF] )
     \\ strip_tac
     \\ simp[evaluate_append]
     \\ imp_res_tac calls_length
@@ -2189,22 +2221,43 @@ val calls_correct = Q.store_thm("calls_correct",
     \\ rveq \\ fs[]
     \\ reverse BasicProvers.TOP_CASE_TAC \\ fs[]
     >- (
-      rw[]
+      rw[] \\ fs[]
+      \\ simp[RIGHT_EXISTS_IMP_THM,RIGHT_EXISTS_AND_THM]
+      \\ strip_tac \\ fs[] \\ rfs[]
+      \\ `code_includes (SND g') t0.code` by metis_tac[code_includes_subg]
+      \\ fs[] \\ rfs[]
+      \\ imp_res_tac evaluate_const \\ fs[]
+      \\ qpat_assum`_ ⇒ _`mp_tac
+      \\ impl_tac
+      >- (
+        fsrw_tac[ETA_ss][env_rel_def,fv1_thm,EXISTS_MAP]
+        \\ metis_tac[] )
+      \\ strip_tac \\ fs[]
       \\ qpat_assum`evaluate(es,env2,_) = _`(mp_tac o MATCH_MP evaluate_add_clock)
       \\ disch_then(qspec_then`ck'`mp_tac) \\ simp[] \\ strip_tac
-      \\ qexists_tac`ck+ck'` \\ simp[]
-      \\ rw[] \\ TRY(Cases_on`e`\\fs[])
-      \\ metis_tac[state_rel_subg,state_rel_def,v_rel_subg])
+      \\ qexists_tac`ck+ck'` \\ simp[])
     \\ strip_tac \\ fs[]
     \\ simp[evaluate_GENLIST_Var]
     \\ imp_res_tac evaluate_length_imp \\ fs[]
     \\ fs[quantHeuristicsTheory.LIST_LENGTH_2] \\ rveq
-    \\ qpat_assum`LENGTH [_] = _`(assume_tac o SYM) \\ fs[]
-    \\ fs[quantHeuristicsTheory.LIST_LENGTH_2] \\ rveq \\ fs[] \\ rveq
+    \\ rfs[] \\ rveq
     \\ first_x_assum drule
     \\ rpt(disch_then drule)
+    \\ simp[RIGHT_EXISTS_IMP_THM,RIGHT_EXISTS_AND_THM,FORALL_AND_THM]
     \\ strip_tac
-    \\ simp[find_code_def]
+    \\ strip_tac \\ fs[] \\ rfs[]
+    \\ `code_includes (SND g') t0.code` by metis_tac[code_includes_subg]
+    \\ fs[]
+    \\ imp_res_tac evaluate_const \\ fs[]
+    \\ qpat_assum`_ ⇒ _`mp_tac
+    \\ impl_keep_tac
+    >- (
+      fsrw_tac[ETA_ss][env_rel_def,fv1_thm]
+      \\ metis_tac[] )
+    \\ strip_tac \\ rveq \\ fs[]
+    \\ first_x_assum drule
+    \\ rpt (disch_then drule)
+    \\ strip_tac \\ fs[]
     \\ `t'.code = t0.code` by (imp_res_tac evaluate_const \\ fs[])
     \\ imp_res_tac evaluate_length_imp \\ fs[] \\ rw[]
     \\ qmatch_assum_rename_tac`LIST_REL (v_rel g1 l1) ev1 ev2`
@@ -2219,7 +2272,7 @@ val calls_correct = Q.store_thm("calls_correct",
     \\ strip_tac \\ fs[]
     \\ Cases_on`ev2 = []` \\ fs[]
     \\ fs[evaluate_app_rw]
-    \\ qpat_assum`_ = (res',_)`mp_tac
+    \\ qpat_assum`_ _ _ _ = (_,_)`mp_tac
     \\ imp_res_tac state_rel_clock \\ fs[]
     \\ imp_res_tac LIST_REL_LENGTH \\ fs[]
     \\ `ALOOKUP (SND g) (x+1) = ALOOKUP (SND g1) (x+1)`
@@ -2243,9 +2296,7 @@ val calls_correct = Q.store_thm("calls_correct",
       \\ strip_tac \\ rveq
       \\ qpat_assum`evaluate(es,env2,_) = _`(mp_tac o MATCH_MP evaluate_add_clock)
       \\ disch_then(qspec_then`ck'`mp_tac) \\ simp[] \\ strip_tac
-      \\ qexists_tac`ck+ck'` \\ simp[]
-      \\ match_mp_tac state_rel_with_clock
-      \\ metis_tac[state_rel_subg])
+      \\ qexists_tac`ck+ck'` \\ simp[find_code_def])
     \\ simp[Once dec_clock_def]
     \\ simp[evaluate_def,evaluate_GENLIST_Var]
     \\ simp[find_code_def]
@@ -2258,10 +2309,7 @@ val calls_correct = Q.store_thm("calls_correct",
       \\ fs[] \\ strip_tac
       \\ qpat_assum`evaluate(es,env2,_) = _`(mp_tac o MATCH_MP evaluate_add_clock)
       \\ disch_then(qspec_then`ck'`mp_tac) \\ simp[] \\ strip_tac
-      \\ qexists_tac`ck+ck'` \\ simp[]
-      \\ fs[dec_clock_def]
-      \\ match_mp_tac (GEN_ALL state_rel_subg)
-      \\ fs[] \\ metis_tac[] )
+      \\ qexists_tac`ck+ck'` \\ simp[])
     \\ fs[NOT_LESS,NOT_LESS_EQUAL]
     \\ strip_tac
     \\ fs[dec_clock_def,TAKE_APPEND1]
@@ -2281,22 +2329,11 @@ val calls_correct = Q.store_thm("calls_correct",
     \\ qpat_assum`evaluate([_],env2,_) = _`(mp_tac o MATCH_MP evaluate_add_clock)
     \\ disch_then(qspec_then`ck''`mp_tac) \\ simp[] \\ strip_tac
     \\ simp[TAKE_APPEND1]
-    \\ qpat_assum`_ = (res',_)`mp_tac
+    \\ qpat_assum`_ _ _ = (_,t'')`mp_tac
     \\ BasicProvers.TOP_CASE_TAC \\ fs[]
     \\ BasicProvers.TOP_CASE_TAC \\ fs[]
     \\ TRY BasicProvers.TOP_CASE_TAC \\ fs[]
-    \\ strip_tac \\ rveq \\ fs[]
-    \\ TRY (Cases_on`res`\\fs[])
-    \\ rveq \\ fs[]
-    \\ TRY (
-      pop_assum mp_tac \\ CASE_TAC \\ fs[]
-      \\ strip_tac \\ rveq \\ fs[] \\ rveq \\ fs[])
-    \\ imp_res_tac evaluate_const \\ fs[]
-    \\ rpt conj_tac
-    \\ TRY(match_mp_tac (GEN_ALL state_rel_subg))
-    \\ TRY(match_mp_tac (GEN_ALL (MP_CANON LIST_REL_mono)))
-    \\ TRY (Cases_on`e''` \\ fs[])
-    \\ metis_tac[v_rel_subg])
+    \\ TRY BasicProvers.TOP_CASE_TAC \\ fs[])
   (* Tick *)
   \\ conj_tac >- cheat
    (*
@@ -2314,27 +2351,30 @@ val calls_correct = Q.store_thm("calls_correct",
     \\ strip_tac \\ asm_exists_tac \\ fs []) *)
   (* Call *)
   \\ conj_tac >- (
-    rw[evaluate_def,calls_def]
+    rw[evaluate_def,calls_def,code_locs_def,ALL_DISTINCT_APPEND]
     \\ pairarg_tac \\ fs[]
     \\ qpat_assum`_ = (res,s)`mp_tac
     \\ BasicProvers.TOP_CASE_TAC \\ fs[]
+    \\ rveq \\ fs[]
     \\ `r.code = FEMPTY`
     by (
       imp_res_tac evaluate_const
-      \\ fs[state_rel_def])
+      \\ fs[wfv_state_def])
     \\ BasicProvers.TOP_CASE_TAC \\ fs[]
     >- ( simp[find_code_def] )
     \\ strip_tac \\ rveq \\ rfs[]
     \\ rw[evaluate_def]
     \\ first_x_assum drule
-    \\ fs[code_locs_def]
+    \\ disch_then drule \\ fs[]
+    \\ simp[RIGHT_EXISTS_IMP_THM,RIGHT_EXISTS_AND_THM,FORALL_AND_THM]
+    \\ strip_tac \\ fs[] \\ strip_tac \\ fs[]
     \\ `env_rel (v_rel g1 l1) env env2 0 (MAP (λx. (0,x)) xs')`
     by ( fsrw_tac[ETA_ss][env_rel_def,fv1_thm,EXISTS_MAP,fv_exists] )
-    \\ disch_then drule \\ fs[]
+    \\ first_x_assum drule
     \\ rpt(disch_then drule) \\ rw[]
     \\ qexists_tac`ck`
     \\ rw[] )
-  \\ conj_tac >- ( rw[evaluate_def] \\ qexists_tac`0` \\ rw[] )
+  \\ conj_tac >- ( rw[evaluate_def] \\ qexists_tac`0` \\ rw[RIGHT_EXISTS_IMP_THM,RIGHT_EXISTS_AND_THM] )
   (* app cons *)
   \\ simp[evaluate_def]
   \\ rpt gen_tac \\ strip_tac
@@ -2343,6 +2383,20 @@ val calls_correct = Q.store_thm("calls_correct",
   >- (
     simp[PULL_EXISTS]
     \\ rpt gen_tac \\ strip_tac
+    \\ simp[RIGHT_EXISTS_AND_THM,RIGHT_EXISTS_IMP_THM]
+    \\ conj_asm1_tac
+    >- (
+      every_case_tac \\ fs[] \\ rveq \\ fs[]
+      \\ match_mp_tac (GEN_ALL dest_closure_wfv)
+      \\ asm_exists_tac \\ fs[] )
+    \\ conj_asm1_tac
+    >- (
+      every_case_tac \\ fs[] \\ rveq \\ fs[]
+      \\ fs[wfv_state_def,dec_clock_def] )
+    \\ qmatch_goalsub_rename_tac`aaa = _ ::_`
+    \\ Cases_on`aaa` \\ fs[]
+    \\ simp[RIGHT_EXISTS_IMP_THM,RIGHT_EXISTS_AND_THM]
+    \\ strip_tac
     \\ simp[evaluate_app_rw]
     \\ drule (GEN_ALL dest_closure_v_rel)
     \\ disch_then drule \\ fs[PULL_EXISTS]
@@ -2353,8 +2407,21 @@ val calls_correct = Q.store_thm("calls_correct",
     \\ imp_res_tac LIST_REL_LENGTH
     \\ rw[] \\ fs[] \\ rw[dec_clock_def]
     \\ match_mp_tac state_rel_with_clock \\ fs[] )
+(*
+
   \\ fs[PULL_EXISTS]
   \\ rpt gen_tac \\ strip_tac
+  \\ simp[RIGHT_EXISTS_AND_THM,RIGHT_EXISTS_IMP_THM]
+  \\ conj_asm1_tac
+  >- (
+    every_case_tac \\ fs[] \\ rveq \\ fs[]
+    \\ match_mp_tac (GEN_ALL dest_closure_wfv)
+    \\ asm_exists_tac \\ fs[] )
+  \\ conj_asm1_tac
+  >- (
+    every_case_tac \\ fs[] \\ rveq \\ fs[]
+    \\ fs[wfv_state_def,dec_clock_def] )
+
   \\ simp[evaluate_app_rw]
   \\ drule (GEN_ALL dest_closure_v_rel)
   \\ disch_then drule \\ fs[PULL_EXISTS]
@@ -2560,6 +2627,7 @@ val calls_correct = Q.store_thm("calls_correct",
   \\ imp_res_tac evaluate_length_imp
   \\ fs[quantHeuristicsTheory.LIST_LENGTH_2]
   \\ rveq \\ strip_tac
+  *)
   \\ cheat);
 
 (*
